# baseURI: https://www.gov.uk/def/ords
# imports: https://purl.org/dc/terms/
# imports: http://www.w3.org/2004/02/skos/core
# prefix: ords

@prefix ords: <https://www.gov.uk/def/ords/> .
@prefix dct: <https://purl.org/dc/terms/> .
@prefix dctype: <https://purl.org/dc/dcmitype/> .
@prefix foaf: <https://xmlns.com/foaf/0.1/> .
@prefix owl: <https://www.w3.org/2002/07/owl#> .
@prefix rdf: <https://www.w3.org/1999/02/22-rdf-syntax-ns#> .
@prefix rdfs: <https://www.w3.org/2000/01/rdf-schema#> .
@prefix skos: <https://www.w3.org/2004/02/skos/core#> .
@prefix xsd: <https://www.w3.org/2001/XMLSchema#> .

<https://www.gov.uk/def/ords>
  a owl:Ontology ;
  dct:license <https://www.nationalarchives.gov.uk/doc/open-government-licence/version/3> ;
  dct:modified "2023-12-11"^^xsd:date ;
  rdfs:comment "ORDS is an RDF vocabulary designed to provide a common set of metadata to describe documents published online by regulatory organisations. Publishing ORDS metadata for online documents regulators increases discoverability and enables data re-users to more easily combine data from multiple regulatory sources."@en ;
  rdfs:label "The Open Reulation Document Standard"@en ;
  owl:imports dct: ;
  owl:imports <https://www.w3.org/2004/02/skos/core> ;
 .

:languageScheme a skos:ConceptScheme ;
    skos:prefLabel "Language"@en ;
    skos:note "A controlled vocabulary for the labnguage of regulatory documents."@en .

:engLanguage a skos:Concept ;
    skos:inScheme :languageScheme ;
    skos:prefLabel "eng"@en ;
    skos:definition "Document is written in the English language." .
 
:cymLanguage a skos:Concept ;
    skos:inScheme :languageScheme ;
    skos:prefLabel "cym"@en ;
    skos:definition "Document is written in the Welsh language." .

:formatScheme a skos:ConceptScheme ;
    skos:prefLabel "Format"@en ;
    skos:note "A controlled vocabulary for the format of regulatory documents."@en .

:pdfFormat a skos:Concept ;
    skos:inScheme :formatScheme ;
    skos:prefLabel "PDF"@en ;
    skos:definition "Document is in PDF format." .
 
:htmlFormat a skos:Concept ;
    skos:inScheme :formatScheme ;
    skos:prefLabel "HTML"@en ;
    skos:definition "Document is in HTML format." .

:wordFormat a skos:Concept ;
    skos:inScheme :formatScheme ;
    skos:prefLabel "MS Word"@en ;
    skos:definition "Document is in an MS Word format." .

:odfFormat a skos:Concept ;
    skos:inScheme :formatScheme ;
    skos:prefLabel "ODF"@en ;
    skos:definition "Document is in Open Document Format (ODF)." .

:odtFormat a skos:Concept ;
    skos:inScheme :formatScheme ;
    skos:prefLabel "ODT"@en ;
    skos:definition "Document is in an ODT format." .

:richTextFormat a skos:Concept ;
    skos:inScheme :formatScheme ;
    skos:prefLabel "Rich Text"@en ;
    skos:definition "Document is in a Rich Text format." .

:typeScheme a skos:ConceptScheme ;
    skos:prefLabel "Type"@en ;
    skos:note "A controlled vocabulary for the legal type of regulatory documents."@en .

:guidanceType a skos:Concept ;
    skos:inScheme :typeScheme ;
    skos:prefLabel "Guidance"@en ;
    skos:definition "Document is regulatory guidance." .

:statutoryGuidanceType a skos:Concept ;
    skos:inScheme :typeScheme ;
    skos:prefLabel "Statutory Guidance"@en ;
    skos:definition "Document is statutory guidance." .

:legislationType a skos:Concept ;
    skos:inScheme :typeScheme ;
    skos:prefLabel "Legislation"@en ;
    skos:definition "Document is legislation." .

:standardType a skos:Concept ;
    skos:inScheme :typeScheme ;
    skos:prefLabel "Standard"@en ;
    skos:definition "Document is a standard." .

:statusScheme a skos:ConceptScheme ;
    skos:prefLabel "Status"@en ;
    skos:note "A controlled vocabulary to denote whether the document is in force."@en .

:activeStatus a skos:Concept ;
    skos:inScheme :statusScheme ;
    skos:prefLabel "Active"@en ;
    skos:definition "Document is active and in force." .

:notActiveStatus a skos:Concept ;
    skos:inScheme :statusScheme ;
    skos:prefLabel "Not Active"@en ;
    skos:definition "Document is not active nor in force." .

:supersededStatus a skos:Concept ;
    skos:inScheme :statusScheme ;
    skos:prefLabel "Superseded"@en ;
    skos:definition "Document has been superseded by another document." .

:subjectScheme a skos:ConceptScheme ;
    skos:prefLabel "Subject"@en ;
    skos:note "A controlled vocabulary for the sector(s) that the document pertains to."@en .

:agricultureForestryAndFishingSubject a skos:Concept ;
    skos:inScheme :subjectScheme ;
    skos:prefLabel "Agriculture, Forestry and Fishing"@en ;
    skos:definition "Activities related to the cultivation of crops, livestock farming, forestry, logging, fishing (wild capture and aquaculture), and rural land management." .

:miningAndQuarryingSubject a skos:Concept ;
    skos:inScheme :subjectScheme ;
    skos:prefLabel "Mining and Quarrying"@en ;
    skos:definition "Involves the extraction of minerals, oil, gas, coal, stone, and other geological materials from the earth." .

:manufacturingSubject a skos:Concept ;
    skos:inScheme :subjectScheme ;
    skos:prefLabel "Manufacturing"@en ;
    skos:definition "The production of goods through the transformation of raw materials or components, and assembly of products across various industries." .


:constructionSubject a skos:Concept ;
    skos:inScheme :subjectScheme ;
    skos:prefLabel "Construction"@en ;
    skos:definition "Encompasses the building of infrastructure (residential, commercial, and industrial buildings), roads, bridges, and other physical structures." .

:utilitiesSubject a skos:Concept ;
    skos:inScheme :subjectScheme ;
    skos:prefLabel "Utilities"@en ;
    skos:definition "Provision of essential services such as electricity, gas, water supply and waste management." .

:realEstateSubject a skos:Concept ;
    skos:inScheme :subjectScheme ;
    skos:prefLabel "Real Estate"@en ;
    skos:definition "Activities including property development, buying, selling, leasing, and managing residential, commercial, and industrial properties." .

:wholesaleRetailAndConsumerServicesSubject a skos:Concept ;
    skos:inScheme :subjectScheme ;
    skos:prefLabel "Wholesale, Retail and Consumer Services"@en ;
    skos:definition "Wholesale involves selling goods in bulk to businesses, while retail includes selling products and services directly to consumers. Consumer services cover areas such as repairs, cleaning and personal care." .

:foodAndDrinkSubject a skos:Concept ;
    skos:inScheme :subjectScheme ;
    skos:prefLabel "Food and Drink"@en ;
    skos:definition "Covers production, processing, distribution, and retail of food and beverages, including restaurants and catering services." .

:accommodationTourismAndLeisureSubject a skos:Concept ;
    skos:inScheme :subjectScheme ;
    skos:prefLabel "Accommodation, Tourism and Leisure"@en ;
    skos:definition "Includes businesses providing lodging and related services, tourist sites, and leisure activities." .

:mediaAndCreativeIndustriesSubject a skos:Concept ;
    skos:inScheme :subjectScheme ;
    skos:prefLabel "Media and Creative Industries"@en ;
    skos:definition "Involves the creation, production and distribution of content in areas such as publishing, film, television, music, and digital media." .

:transportationAndStorageSubject a skos:Concept ;
    skos:inScheme :subjectScheme ;
    skos:prefLabel "Transportation and Storage"@en ;
    skos:definition "Encompasses the movement of goods and people through land, sea and air transportation services, as well as warehousing and logistics operations." .

:financialAndProfessionalServicesSubject a skos:Concept ;
    skos:inScheme :subjectScheme ;
    skos:prefLabel "Financial and Professional Services"@en ;
    skos:definition "Includes banking, insurance, accounting, legal services, consultancy, IT and other financial or advisory services." .

:educationAndTrainingSubject a skos:Concept ;
    skos:inScheme :subjectScheme ;
    skos:prefLabel "Education and Training"@en ;
    skos:definition "Involves institutions providing academic, vocational, and professional education, as well as training services for workforce development." .

:healthSubject a skos:Concept ;
    skos:inScheme :subjectScheme ;
    skos:prefLabel "Health"@en ;
    skos:definition "Covers medical and healthcare services provided by hospitals, clinics, and other organisations including pharmaceuticals and biotechnology." .

:scientificResearchInnovationAndTechnologySubject a skos:Concept ;
    skos:inScheme :subjectScheme ;
    skos:prefLabel "Scientific Research, Innovation and Technology"@en ;
    skos:definition "Covers the research activities across technology, engineering and emerging industries such as AI." .

:generalBusinessRegulationsSubject a skos:Concept ;
    skos:inScheme :subjectScheme ;
    skos:prefLabel "General Business Regulations"@en ;
    skos:definition "Refers to the overarching laws and policies that govern business operations, including compliance, labour laws, taxation and trade regulations." .

ords:regulatorDocument
  a rdfs:Class ;
  a owl:Class ;
  rdfs:comment "A document published online by a regulator."@en ;
  rdfs:label "Regulatory Document"@en ;
 .

ords:title
  a rdf:Property ; 
  rdfs:comment "Title of the document."@en ;
  rdfs:label "Title"@en ;
  rdfs:subPropertyOf dct:title ;
.

ords:identifier
  a rdf:Property ; 
  rdfs:comment "An unambiguous reference to the document, usually a stable URL."@en ;
  rdfs:label "Identifier"@en ;
  rdfs:subPropertyOf dct:identifier ;
.

ords:publisher
  a rdf:Property ; 
  rdfs:comment "The organisation responsible for the document."@en ;
  rdfs:label "Publisher"@en ;
  rdfs:subPropertyOf dct:publisher ;
.

ords:language
  a rdf:Property ; 
  rdfs:comment "Language(s) the document is written in."@en ;
  rdfs:label "Language"@en ;
  rdfs:subPropertyOf dct:language ;
.

ords:format
  a rdf:Property ; 
  rdfs:comment "Format of the document, e.g. PDF, HTML"@en ;
  rdfs:label "Format"@en ;
  rdfs:subPropertyOf dct:format ;
  skos:inScheme :formatScheme ;
  rdfs:range skos:Concept .


ords:description
  a rdf:Property ; 
  rdfs:comment "A brief description of the document."@en ;
  rdfs:label "Description"@en ;
  rdfs:subPropertyOf dct:description ;
.

ords:dateIssued
  a rdf:Property ; 
  rdfs:comment "Date that the document was formally issued."@en ;
  rdfs:label "Date Issued"@en ;
  rdfs:subPropertyOf dct:issued ;
.

ords:dateModified
  a rdf:Property ; 
  rdfs:comment "Date when the document was (last) changed."@en ;
  rdfs:label "Date Modified"@en ;
  rdfs:subPropertyOf dct:modified ;
.

ords:dateValid
  a rdf:Property ; 
  rdfs:comment "Date  when the document is valid. This will be the most recent of date_issued and date_modified."@en ;
  rdfs:label "Date Valid"@en ;
  rdfs:subPropertyOf dct:valid ;
.

ords:audience
  a rdf:Property ; 
  rdfs:comment "People or organisations that this document is intended for."@en ;
  rdfs:label "Audience"@en ;
  rdfs:subPropertyOf dct:audience ;
.

ords:coverage
  a rdf:Property ; 
  rdfs:comment "The jurisdiction(s) under which the document is relevant."@en ;
  rdfs:label "Coverage"@en ;
  rdfs:subPropertyOf dct:coverage ;
.

ords:subject
  a rdf:Property ; 
  rdfs:comment "Sector(s) covering the document's business area."@en ;
  rdfs:label "Subject"@en ;
  rdfs:subPropertyOf dct:subject ;
  skos:inScheme :subjectScheme ;
  rdfs:range skos:Concept .

ords:type
  a rdf:Property ; 
  rdfs:comment "Categorisation of the type of regulatory document e.g. Guidance, Standard"@en ;
  rdfs:label "Type"@en ;
  rdfs:subPropertyOf dct:type ;
  skos:inScheme :typeScheme ;
  rdfs:range skos:Concept .

ords:type
  a rdf:Property ; 
  rdfs:comment "Categorisation of the type of regulatory document e.g. Guidance, Standard."@en ;
  rdfs:label "Type"@en ;
  rdfs:subPropertyOf dct:type ;
.

ords:license
  a rdf:Property ; 
  rdfs:comment "The licence regulating reuse of the document."@en ;
  rdfs:label "License"@en ;
  rdfs:subPropertyOf dct:license ;
.

ords:regulatoryTopics
  a rdf:Property ;
  a owl:ObjectProperty ; 
  rdfs:comment "The regulatory subject areas of the document."@en ;
  rdfs:label "Regulatory Topics"@en ;
  rdfs:domain ords:regulatorDocument ;
.

ords:status
  a rdf:Property ;
  a owl:ObjectProperty ; 
  rdfs:comment "The legal status of the document. This property is used to distinguish between binding documents and guidance."@en ;
  rdfs:label "Status"@en ;
  rdfs:domain ords:regulatorDocument ;
  skos:inScheme :statusScheme ;
  rdfs:range skos:Concept .

ords:dateUploaded
  a rdf:Property ;
  a owl:DatatypeProperty ;
  rdfs:comment "The date that the document was uploaded to the Open Regulation Platform."@en ;
  rdfs:label "Date Uploaded"@en ;
  rdfs:domain ords:regulatorDocument ;
  rdfs:range xsd:date ;
.

ords:hasFormat
  a rdf:Property ; 
  rdfs:comment "A way to relate versions of a document in different formats, e.g. linking the HTML version with a PDF version, inverse of isFormatOf"@en ;
  rdfs:label "Has Format"@en ;
  rdfs:subPropertyOf dct:hasFormat ;
.

ords:isFormatOf
  a rdf:Property ; 
  rdfs:comment "A way to relate versions of a document in different formats, e.g. linking the HTML version with a PDF version, inverse of hasFormat"@en ;
  rdfs:label "Is Format Of"@en ;
  rdfs:subPropertyOf dct:isFormatOf ;
.

ords:hasVersion
  a rdf:Property ; 
  rdfs:comment "Relating a document to another version, e.g. a new updated version of the document, inverse of isVersionOf"@en ;
  rdfs:label "Has Version"@en ;
  rdfs:subPropertyOf dct:hasVersion ;
.

ords:isVersionOf
  a rdf:Property ; 
  rdfs:comment "Relating a document to another version, e.g. a new updated version of the document, inverse of hasVersion"@en ;
  rdfs:label "Is Version Of"@en ;
  rdfs:subPropertyOf dct:isVersionOf ;
.

ords:references
  a rdf:Property ; 
  rdfs:comment "Relating a cited or referenced document, inverse of isReferencedBy"@en ;
  rdfs:label "References"@en ;
  rdfs:subPropertyOf dct:references ;
.

ords:isReferencedBy
  a rdf:Property ; 
  rdfs:comment "Relating a cited or referenced document, inverse of references"@en ;
  rdfs:label "Is Referenced By"@en ;
  rdfs:subPropertyOf dct:isReferencedBy ;
.

ords:hasPart
  a rdf:Property ; 
  rdfs:comment "A way to relate the whole document to a part of a document, where they are referenced or published separately. Inverse of isPartOf"@en ;
  rdfs:label "Has Part"@en ;
  rdfs:subPropertyOf dct:hasPart ;
.

ords:isPartOf
  a rdf:Property ; 
  rdfs:comment "A way to relate the whole document to a part of a document, where they are referenced or published separately. Inverse of hasPart"@en ;
  rdfs:label "Is Part Of"@en ;
  rdfs:subPropertyOf dct:isPartOf ;
.

ords:isReplacedBy
  a rdf:Property ; 
  rdfs:comment "Relating a document that replaces or supersedes the document. Inverse of replaces"@en ;
  rdfs:label "Is Replaced By"@en ;
  rdfs:subPropertyOf dct:isReplacedBy ;
.

ords:replaces
  a rdf:Property ; 
  rdfs:comment "Relating a document to the old superseded or replaced document, inverse of isReplacedBy"@en ;
  rdfs:label "Replaces"@en ;
  rdfs:subPropertyOf dct:replaces ;
.

ords:relatedLegislation
  a rdf:Property ;
  a owl:DatatypeProperty ;
  rdfs:comment "This property is used to relate a document to the legislation that enables or enforces it"@en ;
  rdfs:label "Related Legislation"@en ;
  rdfs:domain ords:regulatorDocument ;
  rdfs:range xsd:anyURI ;
.  



